Java/src/Logic/ST.v
@@ -13,20 +13,12 @@ Inductive ST : Type :=
 
 Definition STs := Map [stptr, ST].
 
-Definition singleton_STs (x : var) (st: open ST) : open STs := fun s => add (val_to_stptr (s x)) (st s) (empty _).
-
 Fixpoint subst_ST (x : var) (v : val) (t : ST) : ST :=
   match t with
   | st_end => st_end
   | st_send x' A t' => st_send x' (apply_subst A (subst1 `v x)) (subst_ST x v t')
   | st_recv x' A t' => st_recv x' (apply_subst A (subst1 `v x)) (subst_ST x v t')
   end.
-
-Definition prune_STs (x : var) (st: open STs) : open STs := fun s => 
-	match (s x) with
-	  | vst c => remove c (st s)
-	  | _ => st s
-	end.
 
 Definition subst_STs (x : var) (v : val) (t : STs) : STs := map (subst_ST x v) t.
 
@@ -86,11 +78,15 @@ Proof.
       + admit (* fangel *).
 Qed.
 
-Definition STs_traces (P : Prog_wf) (t : STs) (tr : traces) : Prop := forall k t', MapsTo k t' t -> exists tr', MapsTo k tr' tr /\ ST_trace P (remove k tr) t' tr'.
-
+Definition STs_traces (P : Prog_wf) (t : STs) (tr : traces) : Prop := forall k t', 
+  MapsTo k t' t -> exists tr', MapsTo k tr' tr /\ ST_trace P (remove k tr) t' tr'.
 
 Program Definition has_ST (c : val) (t : ST) : tasn := 
-  mk_tasn (fun trs => mk_asn (fun P k h => forall P' tr, Prog_wf_sub P P' -> MapsTo (val_to_stptr c) tr trs -> ST_trace P' (remove (val_to_stptr c) trs) t tr) _ _ _) _.
+  mk_tasn (fun trs => mk_asn (fun P k h => forall P' tr, 
+    Prog_wf_sub P P' -> 
+    MapsTo (val_to_stptr c) tr trs -> 
+    ST_trace P' (remove (val_to_stptr c) trs) t tr
+  ) _ _ _) _.
 Next Obligation.
   assert (Prog_wf_sub P P'0).
     transitivity P'; assumption.
@@ -103,9 +99,7 @@ Next Obligation.
 Defined.
 
 Module STNotations.
- 
-	(* Notation " x ':' t " := (singleton_STs x t) (at level 88, left associativity) : st_scope. *)
- 
+  
 	Notation " x ':' t " := (has_ST x t) (at level 88, left associativity) : st_scope.
 
 	Notation " '!' x ',{' P '}.' t " := (st_send x P t) (at level 88, left associativity) : st_scope.
